Automata/Projection.lean
@@ -5,6 +5,7 @@ import Automata.DFA
 import Automata.NFA
 import Automata.Input
 import Automata.Addition
+import Automata.Replicate
 
 
 -- Auxilliary theorems for recover
@@ -18,7 +19,7 @@ def recover (m : Fin (n + 1)) (x: Fin (b+2)):
     fun i => fun j => if h1: j.val < m.val then i ⟨j.val, finLt m j.val h1⟩
       else if h2: j.val > m.val then i ⟨j.val - 1, finPred m j h2⟩ else x
 
-def project (dfa : DFA (Fin (n+1) → Fin (b+2)) state) (m : Fin (n+1)) [DecidableEq state] :
+def project (m : Fin (n+1)) (dfa : DFA (Fin (n+1) → Fin (b+2)) state) [DecidableEq state] :
   NFA (Fin n → Fin (b+2)) state := {
   transition :=
   fun a q => ⟨(List.map (fun (x : Fin (b+2)) => dfa.transition (recover m x a) q)
@@ -27,33 +28,52 @@ def project (dfa : DFA (Fin (n+1) → Fin (b+2)) state) (m : Fin (n+1)) [Decidab
   output := dfa.output
 }
 
+#eval [(fun _ => 0 : Fin 2 → Fin (0 + 2)), fun _ => 1]
 -- Problem: exists x, 1 + 1 = x?
-#eval (project (addBase 2)  2).eval [fun _ => 1]
+#eval (project 2 (addBase 2)).eval [fun _ => 1]
 -- Fix:
-#eval (project (addBase 2) 2).eval [fun _ => 0, fun _ => 1]
+#eval (project 2 (addBase 2)).eval [fun _ => 0, fun _ => 1]
 
-theorem DFAO.bounded_out [Fintype state] (dfao : DFAO (Fin n → Fin (b+2)) state out) (x : List (Fin n → Fin (b+2))) (o: out)(h: ∀ (x : List (Fin n → Fin (b+2))), dfao.eval x = o → (∀ y, (∃ m, y = (List.replicate m (fun _ => 0)) ++ x) →  dfao.eval y = o)) : ∀ z, (∃ k, z = (List.replicate k (fun _ => 0)) ++ x) ∧ dfao.eval z = o → dfao.eval (List.replicate (Fintype.card state) (fun _ => 0) ++ x) = o := by
-  rintro z ⟨⟨k, hz⟩, hzo⟩
+#eval (project 2 (addBase 2)).eval (inputToBase 2 (by omega) [100000, 10000])
+
+def padZeroes (m : ℕ) (x : List (Fin n → Fin (b+2))) : List (Fin n → Fin (b+2)) :=
+  List.replicate m (fun _ => 0) ++ x
+
+theorem padZeroes_add (a b : ℕ) (x : List (Fin n → Fin (k+2))) : padZeroes a (padZeroes b x) = padZeroes (a + b) x := by
+  simp only [padZeroes]
+  rw[← List.append_assoc, List.replicate_append_add]
+
+theorem padZeroes_length (m : ℕ) (x : List (Fin n → Fin (b+2))) : (padZeroes m x).length = m + x.length := by
+  simp only [padZeroes]
+  rw[List.replicate_append_length]
+
+theorem padZeroes_zero (m i: ℕ) (x : List (Fin n → Fin (b+2))) (h : i < m) : (padZeroes m x)[i]'(by simp only [padZeroes, List.length_append, List.length_replicate]; omega) = fun _ => 0 := by
+  simp only [padZeroes]
+  rwa[List.getElem_of_replicate_append_left]
+
+theorem padZeroes_diff (a b: ℕ) (x y : List (Fin n → Fin (k+2))) (hab : a ≤ b) (h: (padZeroes a x) = (padZeroes b y)) : x = padZeroes (b - a) y := by
+  simp only [padZeroes] at *
+  apply List.eq_diff_of_replicate_append_eq
+  . exact h
+  . exact hab
+
+theorem DFAO.bounded_out [Fintype state] (dfao : DFAO (Fin n → Fin (b+2)) state out) (x : List (Fin n → Fin (b+2))) (o: out)(h: ∀ (x : List (Fin n → Fin (b+2))), dfao.eval x = o → (∀ m, dfao.eval (padZeroes m x) = o)) : ∀ k, dfao.eval (padZeroes k x) = o → dfao.eval (padZeroes (Fintype.card state) x) = o := by
+  rintro k hkxo
   by_cases hkstate : k ≤ Fintype.card state
-  . apply h z
-    . exact hzo
-    . use Fintype.card state - k
-      rw[hz]
-      rw[← List.append_assoc, ← List.replicate_add]
-      subst hzo hz
-      simp only [List.append_cancel_right_eq, List.replicate_inj, or_true, and_true]
-      omega
+  . have: Fintype.card state = (Fintype.card state - k) + k := by omega
+    rw[this, ← padZeroes_add (Fintype.card state - k) k x]
+    apply h
+    exact hkxo
 
   simp only [not_le] at hkstate
   -- Question: How to get this kind of descent argument work in lean?
-  . induction' hk : k - Fintype.card state using Nat.strong_induction_on  with d ih generalizing k z
-    have hzlen : Fintype.card state ≤ z.length := by
-      rw[hz]
-      simp only [List.length_append, List.length_replicate]
+  . induction' hk : k - Fintype.card state using Nat.strong_induction_on  with d ih generalizing k
+    have hkxlen : Fintype.card state ≤ (padZeroes k x).length := by
+      simp only [padZeroes_length]
       omega
 
-    obtain ⟨a, b', c, hzabc, hablen, hne, hy⟩ := dfao.pumping_lemma_eval hzo hzlen
-    have hacl : dfao.eval (a ++ c) = o := by
+    obtain ⟨a, b', c, hkxabc, hablen, hne, hy⟩ := dfao.pumping_lemma_eval hkxo hkxlen
+    have haco : dfao.eval (a ++ c) = o := by
       apply hy
       simp only [Language.mem_mul, exists_exists_and_exists_and_eq_and, List.append_assoc]
       use a, (by exact rfl), [], (by exact Language.nil_mem_kstar {b'}), c, (by exact rfl)
@@ -61,20 +81,14 @@ theorem DFAO.bounded_out [Fintype state] (dfao : DFAO (Fin n → Fin (b+2)) stat
     -- have hblen : 0 < b'.length := by
     --   exact List.length_pos_of_ne_nil hne
 
-    have habzero' : ∀ i, ∀ (hi: i < a.length + b'.length),  z[i]'(by omega) = fun _ => 0 := by
-      intro i hi
-      have hik : i < k := by
-        omega
-      simp only [hz]
-      rw[List.getElem_append_left, List.getElem_replicate]
-      rwa[List.length_replicate]
     have habzero : ∀ i, ∀ (hi: i < a.length + b'.length),  (a ++ b')[i]' (by rw[List.length_append]; exact hi) = fun _ => 0 := by
       intro i hi
       rw[← List.getElem_append_left (a++b') c]
-      trans z[i]
-      . congr; exact hzabc.symm
-      specialize habzero' i hi
-      convert habzero'
+      trans (padZeroes k x)[i]
+      congr 1
+      . exact hkxabc.symm
+      . apply padZeroes_zero k
+        omega
       simp only [List.append_assoc, List.length_append]
       . omega
 
@@ -106,71 +120,207 @@ theorem DFAO.bounded_out [Fintype state] (dfao : DFAO (Fin n → Fin (b+2)) stat
         simp only [List.getElem_replicate]
         exact hbzero n_1 h₁
     have habk : a.length + b'.length < k := by omega
-    have hk : (List.replicate k (fun x : Fin n → Fin (b+2) => 0)) = (List.replicate (a.length + b'.length) (fun x : Fin n → Fin (b+2) => 0)) ++ (List.replicate (k - a.length - b'.length) (fun x : Fin n → Fin (b+2) => 0)) := by
+    have hk : (List.replicate k (fun _ => 0)) = (List.replicate (a.length + b'.length) (fun _ => 0)) ++ (List.replicate (k - a.length - b'.length) (fun _ : Fin n => (0 : Fin (b + 2)))) := by
       simp[List.append_replicate_replicate]
       omega
-    have hcx : c = (List.replicate (k - a.length - b'.length) (fun _ => 0)) ++ x := by
-      rw[har, hbr] at hzabc
-      rw[hzabc] at hz
-      simp only [List.append_replicate_replicate] at hz
-      -- AHhhh! NO!
-      -- rw[hk] at hz
-      have : (List.replicate k fun x ↦ 0) ++ x = (List.replicate (a.length + b'.length) fun x ↦ 0) ++ (List.replicate (k - a.length - b'.length) fun x ↦ 0) ++ x := by
-        congr
-        simp only [List.append_replicate_replicate, List.replicate_inj, or_true, and_true]
-        omega
-      rw[this, List.append_assoc] at hz
-      exact List.append_cancel_left hz
-
-    have hac : a ++ c = List.replicate (k - b'.length) (fun _ => 0) ++ x := by
+    have hcx : c = padZeroes (k - a.length - b'.length) x := by
+      rw[har, hbr] at hkxabc
+      rw[List.append_assoc, ← padZeroes, ← padZeroes, padZeroes_add] at hkxabc
+      simp only [padZeroes] at hkxabc
+      have : c = padZeroes (k - (a.length + b'.length)) x := by
+        apply List.eq_diff_of_replicate_append_eq
+        . exact hkxabc.symm
+        . omega
+      rw[this]
+      convert rfl using 2
+      omega
+    have hac : a ++ c = padZeroes (k - b'.length) x := by
       rw[hcx, har]
+      simp only [padZeroes, List.length_replicate]
       rw[← List.append_assoc]
       simp only [List.length_replicate, List.append_replicate_replicate,
         List.append_cancel_right_eq, List.replicate_inj, AddLeftCancelMonoid.add_eq_zero,
         List.length_eq_zero, or_true, and_true]
       omega
+
     by_cases hkb : k - b'.length ≤ Fintype.card state
-    . apply h (a ++ c)
-      . exact hacl
-      . -- subst/rw hac !!!
-        use Fintype.card state - (k - b'.length)
-        simp only [hac]
-        rw[← List.append_assoc]
-        simp only [List.append_replicate_replicate, List.append_cancel_right_eq, List.replicate_inj,
-          or_true, and_true]
-        omega
+    . have : Fintype.card state = (Fintype.card state - (k - b'.length)) + (k - b'.length) := by omega
+      rw[this, ← padZeroes_add (Fintype.card state - (k - b'.length)) (k - b'.length) x, ← hac]
+      apply h (a ++ c)
+      . exact haco
     . simp only [not_le] at hkb
       have hblen : 0 < b'.length := by
         exact List.length_pos_of_ne_nil hne
 
-      specialize ih (k - b'.length - Fintype.card state) (by omega) (a ++ c) (hacl) (k - b'.length) hac hkb rfl
+      specialize ih (k - b'.length - Fintype.card state) (by omega) (k - b'.length)
+      apply ih
+      . rw[← hac]
+        exact haco
+      . exact hkb
+      . rfl
 
-      exact ih
-
-theorem DFA.bounded_accept [Fintype state] (dfa : DFA (Fin n → Fin (b+2)) state) (x : List (Fin n → Fin (b+2)))(h: ∀ (x : List (Fin n → Fin (b+2))), dfa.eval x→ (∀ y, (∃ m, y = (List.replicate m (fun _ => 0)) ++ x) →  dfa.eval y)) : ∀ z, (∃ k, z = (List.replicate k (fun _ => 0)) ++ x) ∧ dfa.eval z → dfa.eval (List.replicate (Fintype.card state) (fun _ => 0) ++ x) := by
+theorem DFA.bounded_accept [Fintype state] (dfa : DFA (Fin n → Fin (b+2)) state) (x : List (Fin n → Fin (b+2)))(h: ∀ (x : List (Fin n → Fin (b+2))), dfa.eval x→ (∀ m, dfa.eval (padZeroes m x))): ∀ z, (∃ k, z = padZeroes k x) ∧ dfa.eval z → dfa.eval (padZeroes (Fintype.card state) x) := by
   have := DFAO.bounded_out dfa x true
   intro z a
-  simp_all only [forall_exists_index, and_imp]
+  simp_all only [implies_true, true_implies]
   obtain ⟨left, right⟩ := a
   obtain ⟨w, h_1⟩ := left
   subst h_1
   apply this
-  · intro x_1 a y x_2 h_1
-    subst h_1
-    apply h
-    · simp_all only
-    · rfl
-  · rfl
   · exact right
 
-theorem NFA.bounded_accept [Fintype state] [DecidableEq state] (nfa : NFA (Fin n → Fin (b+2)) state) (x : List (Fin n → Fin (b+2)))(h: ∀ (x : List (Fin n → Fin (b+2))), nfa.eval x→ (∀ y, (∃ m, y = (List.replicate m (fun _ => 0)) ++ x) →  nfa.eval y)) : ∀ z, (∃ k, z = (List.replicate k (fun _ => 0)) ++ x) ∧ nfa.eval z → nfa.eval (List.replicate (Fintype.card (ListND state)) (fun _ => 0) ++ x) := by
+theorem NFA.bounded_accept [Fintype state] [DecidableEq state] (nfa : NFA (Fin n → Fin (b+2)) state) (x : List (Fin n → Fin (b+2)))(h: ∀ (x : List (Fin n → Fin (b+2))), nfa.eval x→ (∀ m, nfa.eval (padZeroes m x))): ∀ z, (∃ k, z = padZeroes k x) ∧ nfa.eval z → nfa.eval (padZeroes (Fintype.card (ListND state)) x) := by
   simp only [← NFA.toDFA_eval] at *
   have := DFA.bounded_accept (nfa.toDFA) x h
   intro z a
-  simp_all only [forall_exists_index, and_imp]
+  simp_all only [and_imp, forall_exists_index]
   obtain ⟨left, right⟩ := a
   obtain ⟨w, h_1⟩ := left
   subst h_1
   apply this
   · rfl
   · exact right
+
+
+
+-- Old version
+-- theorem DFAO.bounded_out [Fintype state] (dfao : DFAO (Fin n → Fin (b+2)) state out) (x : List (Fin n → Fin (b+2))) (o: out)(h: ∀ (x : List (Fin n → Fin (b+2))), dfao.eval x = o → (∀ y, (∃ m, y = padZeroes m x) →  dfao.eval y = o)) : ∀ z, (∃ k, z = (padZeroes k x)) ∧ dfao.eval z = o → dfao.eval (padZeroes (Fintype.card state) x) = o := by
+--   simp only [padZeroes]
+--   rintro z ⟨⟨k, hz⟩, hzo⟩
+--   by_cases hkstate : k ≤ Fintype.card state
+--   . apply h z
+--     . exact hzo
+--     . use Fintype.card state - k
+--       rw[hz]
+--       simp only [padZeroes]
+--       rw[← List.append_assoc, ← List.replicate_add]
+--       subst hzo hz
+--       simp only [List.append_cancel_right_eq, List.replicate_inj, or_true, and_true]
+--       omega
+
+--   simp only [not_le] at hkstate
+--   -- Question: How to get this kind of descent argument work in lean?
+--   . induction' hk : k - Fintype.card state using Nat.strong_induction_on  with d ih generalizing k z
+--     have hzlen : Fintype.card state ≤ z.length := by
+--       rw[hz]
+--       simp only [List.length_append, List.length_replicate]
+--       omega
+
+--     obtain ⟨a, b', c, hzabc, hablen, hne, hy⟩ := dfao.pumping_lemma_eval hzo hzlen
+--     have haco : dfao.eval (a ++ c) = o := by
+--       apply hy
+--       simp only [Language.mem_mul, exists_exists_and_exists_and_eq_and, List.append_assoc]
+--       use a, (by exact rfl), [], (by exact Language.nil_mem_kstar {b'}), c, (by exact rfl)
+--       simp only [List.nil_append]
+--     -- have hblen : 0 < b'.length := by
+--     --   exact List.length_pos_of_ne_nil hne
+
+--     have habzero' : ∀ i, ∀ (hi: i < a.length + b'.length),  z[i]'(by omega) = fun _ => 0 := by
+--       intro i hi
+--       have hik : i < k := by
+--         omega
+--       simp only [hz]
+--       rw[List.getElem_append_left, List.getElem_replicate]
+--       rwa[List.length_replicate]
+--     have habzero : ∀ i, ∀ (hi: i < a.length + b'.length),  (a ++ b')[i]' (by rw[List.length_append]; exact hi) = fun _ => 0 := by
+--       intro i hi
+--       rw[← List.getElem_append_left (a++b') c]
+--       trans z[i]
+--       . congr; exact hzabc.symm
+--       specialize habzero' i hi
+--       convert habzero'
+--       simp only [List.append_assoc, List.length_append]
+--       . omega
+
+--     have hazero : ∀ i, ∀ (hi: i < a.length),  a[i]' (by omega) = fun _ => 0 := by
+--       intro i hi
+--       rw[← List.getElem_append_left a b']
+--       apply habzero i
+--       . omega
+--     have hbzero : ∀ i, ∀ (hi: i < b'.length),  b'[i]' (by omega) = fun _ => 0 := by
+--       intro i hi
+--       -- rw[← List.getElem_append_right' a b'] Why?
+--       have : (a ++ b')[a.length + i]'(by rw[List.length_append]; omega) = b'[i] := by
+--         rw[List.getElem_append_right']
+--         simp only [add_tsub_cancel_left]
+--         omega
+--       rw[← this]
+--       apply habzero (a.length + i)
+--       omega
+--     have har: a = List.replicate a.length (fun _ => 0) := by
+--       apply List.ext_getElem
+--       . simp
+--       . intro n_1 h₁ h₂
+--         simp only [List.getElem_replicate]
+--         exact hazero n_1 h₁
+--     have hbr: b' = List.replicate b'.length (fun _ => 0) := by
+--       apply List.ext_getElem
+--       . simp
+--       . intro n_1 h₁ h₂
+--         simp only [List.getElem_replicate]
+--         exact hbzero n_1 h₁
+--     have habk : a.length + b'.length < k := by omega
+--     have hk : (List.replicate k (fun _ => 0)) = (List.replicate (a.length + b'.length) (fun _ => 0)) ++ (List.replicate (k - a.length - b'.length) (fun _ : Fin n => (0 : Fin (b + 2)))) := by
+--       simp[List.append_replicate_replicate]
+--       omega
+--     have hcx : c = (List.replicate (k - a.length - b'.length) (fun _ => 0)) ++ x := by
+--       rw[har, hbr] at hzabc
+--       rw[hzabc] at hz
+--       simp only [List.append_replicate_replicate] at hz
+--       -- AHhhh! NO!
+--       rw[hk] at hz
+--       rw[List.append_assoc] at hz
+--       exact List.append_cancel_left hz
+
+--     have hac : a ++ c = List.replicate (k - b'.length) (fun _ => 0) ++ x := by
+--       rw[hcx, har]
+--       rw[← List.append_assoc]
+--       simp only [List.length_replicate, List.append_replicate_replicate,
+--         List.append_cancel_right_eq, List.replicate_inj, AddLeftCancelMonoid.add_eq_zero,
+--         List.length_eq_zero, or_true, and_true]
+--       omega
+--     by_cases hkb : k - b'.length ≤ Fintype.card state
+--     . apply h (a ++ c)
+--       . exact haco
+--       . -- subst/rw hac !!!
+--         use Fintype.card state - (k - b'.length)
+--         simp only [hac, padZeroes]
+--         rw[← List.append_assoc]
+--         simp only [List.append_replicate_replicate, List.append_cancel_right_eq, List.replicate_inj,
+--           or_true, and_true]
+--         omega
+--     . simp only [not_le] at hkb
+--       have hblen : 0 < b'.length := by
+--         exact List.length_pos_of_ne_nil hne
+
+--       specialize ih (k - b'.length - Fintype.card state) (by omega) (a ++ c) (haco) (k - b'.length) hac hkb rfl
+
+--       exact ih
+
+-- theorem DFA.bounded_accept [Fintype state] (dfa : DFA (Fin n → Fin (b+2)) state) (x : List (Fin n → Fin (b+2)))(h: ∀ (x : List (Fin n → Fin (b+2))), dfa.eval x→ (∀ y, (∃ m, y = padZeroes m x) →  dfa.eval y)) : ∀ z, (∃ k, z = padZeroes k x) ∧ dfa.eval z → dfa.eval (padZeroes (Fintype.card state) x) := by
+--   have := DFAO.bounded_out dfa x true
+--   intro z a
+--   simp_all only [forall_exists_index, and_imp]
+--   obtain ⟨left, right⟩ := a
+--   obtain ⟨w, h_1⟩ := left
+--   subst h_1
+--   apply this
+--   · intro x_1 a y x_2 h_1
+--     subst h_1
+--     apply h
+--     · simp_all only
+--     · rfl
+--   · rfl
+--   · exact right
+
+-- theorem NFA.bounded_accept [Fintype state] [DecidableEq state] (nfa : NFA (Fin n → Fin (b+2)) state) (x : List (Fin n → Fin (b+2)))(h: ∀ (x : List (Fin n → Fin (b+2))), nfa.eval x→ (∀ y, (∃ m, y = padZeroes m x) →  nfa.eval y)) : ∀ z, (∃ k, z = padZeroes k x) ∧ nfa.eval z → nfa.eval (padZeroes (Fintype.card (ListND state)) x) := by
+--   simp only [← NFA.toDFA_eval] at *
+--   have := DFA.bounded_accept (nfa.toDFA) x h
+--   intro z a
+--   simp_all only [forall_exists_index, and_imp]
+--   obtain ⟨left, right⟩ := a
+--   obtain ⟨w, h_1⟩ := left
+--   subst h_1
+--   apply this
+--   · rfl
+--   · exact right
