Automata/Experiments.lean
@@ -1,0 +1,87 @@
+import Mathlib.Tactic
+import Mathlib.Data.List.Basic
+import Automata.DFA
+import Automata.NFA
+import Automata.Input
+import Automata.Projection
+import Automata.Addition
+
+def Fin.func_pred (f: Fin (n + 1) → α) : Fin n → α :=
+  fun i => f i
+
+def DFAO.transFrom' (dfa : DFAO α state out) (x : Fin n → α) (s : state) : state :=
+  match n with
+    | 0 => s
+    | i+1 => dfa.transition (x i) (dfa.transFrom' (Fin.func_pred x) s)
+
+def DFAO.evalFrom' (dfa : DFAO α state out) (x : Fin n → α) (q : state) : out := dfa.output (dfa.transFrom' x q)
+
+def DFAO.eval' (dfa : DFAO α state out) (x : Fin n → α) : out := dfa.evalFrom' x dfa.start
+
+def NFA.transFrom' (nfa : NFA α state) (x : Fin n → α) (qs : ListND state) [DecidableEq state] : ListND state :=
+  match n with
+    | 0 => qs
+    | i+1 => nfa.transList (x i) (NFA.transFrom' nfa (Fin.func_pred x) qs)
+
+def NFA.evalFrom' (nfa : NFA α state) (x : Fin n → α) (qs : ListND state) [DecidableEq state] : Bool := (nfa.transFrom' x qs).val.any nfa.output
+
+def NFA.eval' (nfa : NFA α state) (x : Fin n → α) [DecidableEq state]: Bool := nfa.evalFrom' x nfa.start
+
+def toBase' (b: ℕ) (n: ℕ) (h : b ≥ 2): List (Fin b) :=
+  (toBase b n).attach.map (fun x => ⟨x.1, (by apply toBase_lt_base b n (by omega); obtain ⟨val, property⟩ := x; simp_all only)⟩)
+
+def toBaseFin (b n: ℕ) (h : b ≥ 2): Fin (toBase' b n h).length → Fin b :=
+  fun i => (toBase' b n h)[i]
+
+def stretchFin (m: ℕ) (h : b ≥ 2) (f : Fin n → Fin b) : Fin (m + n) → Fin b :=
+  fun i => if h1: i.val < m then ⟨0, by omega⟩ else f ⟨i.val - m, (by omega)⟩
+
+def stretchFinTo (m: ℕ) (h : b ≥ 2) (f : Fin n → Fin b) (hmn : m ≥ n) : Fin m → Fin b :=
+  fun i => if h1: i.val < m - n then ⟨0, by omega⟩ else f ⟨i.val - (m - n), (by omega)⟩
+
+def maxFin (b: ℕ) (l: List ℕ) (h: b ≥ 2) : ℕ :=
+  match l with
+    | [] => 0
+    | x::xs => max ((toBase' b x h).length) (maxFin b xs h)
+
+theorem maxFin_max (b: ℕ) (l: List ℕ) (h: b ≥ 2) : ∀ i, i ∈ l → maxFin b l h ≥ (toBase' b i h).length := by
+  intro i hi
+  induction l with
+    | nil => contradiction
+    | cons x xs ih =>
+      rcases hi with hi | hi
+      . simp only [maxFin, le_max_iff, le_refl, true_or]
+      . simp only [maxFin, le_max_iff]
+        right
+        rename_i a
+        apply ih
+        exact a
+
+-- def mapToBaseFin (b: ℕ) (l: List ℕ) (h: b ≥ 2): Fin l.length → (Fin (maxFin b l h) → Fin b) :=
+--   have : ∀ i, ∀ (hi: i < l.length), (maxFin b l h - (toBase' b l[i] h).length + (toBase' b l[i] h).length) = maxFin b l h := by
+--     intro i hi
+--     have := maxFin_max b l h l[i] (by apply List.getElem_mem)
+--     omega
+
+--   fun i => (stretchFin (maxFin b l h - (toBase' b l[i] h).length) h (toBaseFin b l[i] h) : Fin (maxFin b l h) → Fin b)
+
+def mapToBaseFin (b: ℕ) (l: List ℕ) (h: b ≥ 2): Fin l.length → Fin (maxFin b l h) → Fin b :=
+  fun i => (stretchFinTo (maxFin b l h) h (toBaseFin b l[i] h) (by apply maxFin_max; apply List.getElem_mem) : Fin (maxFin b l h) → Fin b)
+
+def toInputFin (b: ℕ) (l: List ℕ) (h: b ≥ 2): Fin (maxFin b l h) → Fin l.length → Fin b :=
+  fun i => fun j => mapToBaseFin b l h j i
+
+def padZero (k : ℕ) (f : Fin m → Fin n → Fin b) (h : b ≥ 2) : Fin (k + m) → Fin n → Fin b :=
+  fun i => fun j => if h: i.val < k then ⟨0, by omega⟩ else f ⟨i.val - k, (by omega)⟩ j
+
+#eval (addBase 10).eval' (toInputFin 10 [1000, 2000, 3000] (by omega))
+
+#eval (toInputFin 2 [1, 1] (by omega))
+#eval (padZero 1 (toInputFin 2 [1, 1] (by omega)) (by omega))
+
+-- Problem: exists x, 1 + 1 = x?
+#eval (project 2 (addBase 2)).eval' (toInputFin 2 [1, 1] (by omega))
+-- Fix:
+#eval (project 2 (addBase 2)).eval' (padZero 1 (toInputFin 2 [1, 1] (by omega)) (by omega))
+
+#eval (project 2 (addBase 2)).eval (inputToBase 2 (by omega) [100000, 10000])
