Automata/Replicate.lean
@@ -1,0 +1,46 @@
+import Mathlib.Tactic
+import Mathlib.Data.List.Basic
+
+theorem List.replicate_append_length (x : List α) : (List.replicate n a ++ x).length = n + x.length := by
+  rw[List.length_append, List.length_replicate]
+
+theorem List.getElem_of_replicate_append_left (x : List α) (h : i < n) : (List.replicate n a ++ x)[i]'(by simp only [List.length_append, List.length_replicate]; omega) = a := by
+  rw[List.getElem_append_left]
+  rw[List.getElem_replicate]
+  simpa only [List.length_replicate]
+
+theorem List.getElem_of_replicate_append_right (x : List α) (h : i < x.length) : (List.replicate n a ++ x)[i + n]'(by simp only [List.length_append, List.length_replicate]; omega) = x[i]'(by omega) := by
+  rw[List.getElem_append_right]
+  . simp only [length_replicate, add_tsub_cancel_right]
+  . simp only [length_replicate, add_lt_iff_neg_right, not_lt_zero', not_false_eq_true]
+  . simpa only [length_replicate, add_tsub_cancel_right]
+
+theorem List.replciate_append_elem (n: ℕ) (l: List ℕ) :
+  x ∈ ((List.replicate n a) ++ l) → x = a ∨ x ∈ l := by
+  intro h
+  simp only [List.mem_append, List.replicate] at h
+  rcases h with (h | h)
+  . left
+    have : x ∈ [a] := List.replicate_subset_singleton n a h
+    simp_all only [mem_replicate, ne_eq, mem_singleton]
+  . right
+    exact h
+
+theorem List.eq_of_replicate_append_eq {x y : List α} (h : List.replicate n a ++ x = List.replicate n a ++ y) : x = y := by
+  induction n with
+  | zero =>
+    rw[List.replicate_zero, List.nil_append] at h
+    exact h
+  | succ n ih =>
+    rw[List.replicate_succ, List.cons_append] at h
+    injection h with h1 h2
+    exact ih h2
+
+theorem List.replicate_append_add (n m : ℕ) (x : List α) : List.replicate n a ++ List.replicate m a ++ x = List.replicate (n + m) a ++ x := by
+  simp only [List.append_replicate_replicate]
+
+theorem List.eq_diff_of_replicate_append_eq {x y : List α} (h : List.replicate m a ++ x = List.replicate n a ++ y) (hmn : m ≤ n) : x = List.replicate (n - m) a ++ y := by
+  have: n = m + (n - m) := by omega
+  rw[this] at h
+  rw[← List.append_replicate_replicate, List.append_assoc] at h
+  apply List.append_cancel_left h
